src/impl/TLS13.Impl.ConnectionState.Queries.fsti
@@ -339,6 +339,29 @@ fn can_receive_encrypted_extensions
                 CL.message_value = M.TlsHandshake (M.EncryptedExtensions ee);
               }))
 
+fn can_send_encrypted_extensions_runtime
+  (c:connection_state)
+  (#st0:erased CS.connection_state)
+  requires connection_exactly c st0
+  returns ok: bool
+  ensures connection_exactly c st0 **
+          pure (ok ==>
+            st0.CS.cs_model.CS.model_control ==
+              CS.ControlHandshaking CS.HsServerHelloSent /\
+            st0.CS.cs_model.CS.model_config.CS.config_role == CS.ServerEndpoint /\
+            Some?
+              st0.CS.cs_model.CS.model_handshake.CS.hs_keys.CS.ks_server_handshake_traffic /\
+            U64.fits (st0.CS.cs_model.CS.model_record.CS.record_write.R.seq + 1) /\
+            B.length st0.CS.cs_model.CS.model_handshake.CS.hs_transcript + 6 <=
+              max_transcript_len /\
+            CS.legal_event
+              st0.CS.cs_model
+              (CS.ConnNetworkEvent {
+                CL.message_direction = CL.Sent;
+                CL.message_value =
+                  M.TlsHandshake (M.EncryptedExtensions { M.negotiated_alpn = None });
+              }))
+
 fn can_receive_certificate
   (c:connection_state)
   (lcert:IM.certificate_msg)
