src/impl/TLS13.Impl.Server.fsti
@@ -79,6 +79,24 @@ let next_local_action_sound
        st.CS.cs_model.CS.model_handshake.CS.hs_keys.CS.ks_master_secret /\
      not (Some?
        st.CS.cs_model.CS.model_handshake.CS.hs_keys.CS.ks_client_application_traffic)
+    | ST.LocalSendEncryptedExtensions ->
+     action.ST.next_local_payload == ST.LocalPayloadNone /\
+     st.CS.cs_model.CS.model_control ==
+       CS.ControlHandshaking CS.HsServerHelloSent /\
+     st.CS.cs_model.CS.model_config.CS.config_role == CS.ServerEndpoint /\
+     Some?
+       st.CS.cs_model.CS.model_handshake.CS.hs_keys.CS.ks_server_handshake_traffic /\
+     U64.fits
+       (st.CS.cs_model.CS.model_record.CS.record_write.R.seq + 1) /\
+     B.length st.CS.cs_model.CS.model_handshake.CS.hs_transcript + 6 <=
+       Bounds.max_transcript_len /\
+     CS.legal_event
+       st.CS.cs_model
+       (CS.ConnNetworkEvent {
+         CL.message_direction = CL.Sent;
+         CL.message_value =
+           M.TlsHandshake (M.EncryptedExtensions { M.negotiated_alpn = None });
+       })
     | _ ->
      False
   else
